lean/Shars/Verification/Simple/Refinement.lean
@@ -4,17 +4,17 @@ import Shars.Verification.Simple.Utils
 import Sha3.Spec
 
 
-def Vector.toBitVec(self: Vector Bool n): BitVec n := (BitVec.ofBoolListLE <| self.toList).cast (by simp)
-def Aeneas.Std.Array.toBitVec{size: Std.Usize}(self: Std.Array Bool size): BitVec (size.val) :=
-  (BitVec.ofBoolListLE <| self.val).cast (by simp)
-def Aeneas.Std.Slice.toBitVec(self: Aeneas.Std.Slice Bool): BitVec self.length :=
-  (BitVec.ofBoolListLE self.val).cast (by simp)
+abbrev List.toBitVec(self: List Bool): BitVec self.length := BitVec.ofBoolListLE self
+abbrev Vector.toBitVec(self: Vector Bool n): BitVec n := self.toList.toBitVec.cast (by simp)
 
+/- def Aeneas.Std.Array.toBitVec{size: Std.Usize}(self: Std.Array Bool size): BitVec (size.val) := -/
+/-   (BitVec.ofBoolListLE <| self.val).cast (by simp) -/
+/- def Aeneas.Std.Slice.toBitVec(self: Aeneas.Std.Slice Bool): BitVec self.length := -/
+/-   (BitVec.ofBoolListLE self.val).cast (by simp) -/
 
 def simple.StateArray.toSpec(self: simple.StateArray): Spec.Keccak.StateArray 6 :=
-  Spec.Keccak.StateArray.ofBitVec <| self.toBitVec.cast (by simp [Spec.w, Spec.b])
+  Spec.Keccak.StateArray.ofBitVec <| self.val.toBitVec.cast (by simp [Spec.w, Spec.b])
 
-
-abbrev Aeneas.Std.Array.toArray{size: Usize}(self: Aeneas.Std.Array α size): _root_.Array α := Array.mk self.val
-abbrev Aeneas.Std.Slice.toArray(self: Aeneas.Std.Slice α): _root_.Array α := Array.mk self.val
+/- abbrev Aeneas.Std.Array.toArray{size: Usize}(self: Aeneas.Std.Array α size): _root_.Array α := Array.mk self.val -/
+/- abbrev Aeneas.Std.Slice.toArray(self: Aeneas.Std.Slice α): _root_.Array α := Array.mk self.val -/
 
